Interp_state ag lemmas proved

theories/CTree/Logic/AG.v
@@ -10,10 +10,12 @@ From CTree Require Import
   CTree.Core
   CTree.Equ
   CTree.SBisim
+  CTree.Interp.State
   CTree.Logic.Trans
   CTree.Logic.CanStep
   Logic.Setoid
   CTree.Logic.AX
+  CTree.Logic.AF
   Logic.Ctl
   Logic.Tactics
   Logic.Kripke.
@@ -148,73 +150,6 @@ Section BindLemmas.
 
   Typeclasses Transparent sbisim.
   Typeclasses Transparent equ.
-  (* [t] satisfies [φ] until it terminates with post-condition [R],
-     then forall x w, R x w -> k x, w satisfies [φ] forever. *)
-  Lemma ag_bind_r{X Y}: forall (t: ctree E X)
-                          w (k: X -> ctree E Y) φ R,
-      <( t, w |= (vis φ) AU (AX done R) )> ->
-      (forall (x: X) w, R x w -> <( {k x}, w |= AG vis φ )>) ->
-      <( {x <- t ;; k x} , w |= AG vis φ )>.
-  Proof.
-    intros.
-    cinduction H.
-    - (* AX done R *)
-      apply ax_done in H as (Hw & x & Heq & H).
-      intros.
-      rewrite Heq, bind_ret_l.
-      specialize (H0 _ _ H);
-        step in H0; remember (k x) as K; destruct H0;
-        try contradiction.
-      destruct H1; subst.
-      next; split; auto; next; split; auto.
-    - (* AG vis φ *)
-      destruct H1, H2; clear H2.
-      destruct H1 as (t' & w' & TR).
-      cbn in TR, H3, H4.
-      cbn in H.
-      rewrite (ctree_eta t).      
-      remember (observe t) as T.
-      remember (observe t') as T'.
-      rewrite ctl_vis in H.
-      clear HeqT t HeqT' t'.
-      induction TR.
-      + rewrite bind_guard.
-        apply ag_guard.
-        rewrite (ctree_eta t).
-        apply IHTR; eauto.
-        * intros t_ w_ TR_.
-          setoid_rewrite ktrans_guard in H3.
-          setoid_rewrite ktrans_guard in H4.
-          now apply H3.
-        * intros t_ w_ TR_.
-          setoid_rewrite ktrans_guard in H3.
-          setoid_rewrite ktrans_guard in H4.
-          now apply H4.
-      + rewrite bind_br.
-        rewrite <- ag_br.
-        split; [auto|intro j].
-        apply H4.
-        apply ktrans_br.
-        exists j; intuition.
-      + rewrite bind_vis.
-        rewrite <- ag_vis with (v:=v).
-        split; auto. 
-        intro x.
-        apply H4.
-        apply ktrans_vis.
-        exists x; intuition.
-      + inv H.
-      + ddestruction H.
-        rewrite bind_ret_l.
-        assert(TR_:[Ret x, Obs e v] ↦ [stuck, Finish e v x])
-          by now apply ktrans_finish.
-        specialize (H4 Ctree.stuck (Finish e v x) TR_).
-        specialize (H3 Ctree.stuck (Finish e v x) TR_).
-        clear TR_.
-        inv H3; inv H2.
-        now apply can_step_stuck in H3.
-  Qed.
-
   Lemma ag_iter_l{X I}: forall (k: I -> ctree E (I + X)) i w (x: I) φ,
       <( {k i}, w |= AG now φ )> ->
       <( {iter k i}, w |= AG now φ )>.
@@ -224,26 +159,13 @@ Section BindLemmas.
     now apply ag_bind_l.
   Qed.
 
-  (* vis φ <--> done Rr *)
-  Lemma ag_iter_step{X I}: forall (k: I -> ctree E (I + X)) w w' (x x': I) φ,
-      <( {k x}, w |= vis φ AU AX done
-                  {fun (lr: I+X) w => lr = inl x' /\ w = w'} )> ->
-      <( {iter k x'}, w' |= AG vis φ )> ->
-      <( {iter k x}, w |= AG vis φ )>.
-  Proof.
-    intros.
-    rewrite sb_unfold_iter.
-    apply ag_bind_r with (R:=fun (lr : I + X) (w : World E) => lr = inl x' /\ w = w'); auto.
-    now intros [l | r] w_ (Hinv & ->); inv Hinv.
-  Qed.
-
   Notation MP X := (rel (ctree E X) (World E)).
-  
-  Program Definition ag_bind_clos{X Y} φ Post : mon (MP Y) :=
+  Program Definition ag_bind_vis_clos{X Y} φ Post : mon (MP Y) :=
     {| body R t w :=
         bind_ctx1
-          (fun (t: ctree E X) => <( t, w |= vis φ AU (AX done Post) )>)
-          (fun (k: X -> ctree E Y) => forall (x: X) w, Post x w -> R (k x) w)
+          (fun (t: ctree E X) => <( t, w |= vis φ AU (AX finish Post) )>)
+          (fun (k: X -> ctree E Y) =>
+             forall (x: X) (e: E) (v: encode e), Post e v x -> R (k x) (Obs e v))
           t
     |}.
   Next Obligation.
@@ -252,123 +174,368 @@ Section BindLemmas.
     apply in_bind_ctx1; eauto.
   Qed.
 
-  Lemma ag_bind_ag{X Y} φ Post:
-      ag_bind_clos (X:=X) (Y:=Y) φ Post <= cart <( |- vis φ )> <( |- ⊥ )>.
+  Lemma ag_bind_vis_ag{X Y} φ Post:
+      ag_bind_vis_clos (X:=X) (Y:=Y) φ Post <= cart <( |- vis φ )> <( |- ⊥ )>.
   Proof.    
     apply Coinduction.
     intros R t w; cbn.
     apply (leq_bind_ctx1 _ _
              (fun t => carF (entailsF <( vis {φ} )>) (entailsF <( ⊥ )>)
                       (carT (entailsF <( vis {φ} )>) (entailsF <( ⊥ )>)
-                         (ag_bind_clos φ Post) R) t w)). 
+                         (ag_bind_vis_clos φ Post) R) t w)). 
     intros x Hx k Hk.
     cinduction Hx.
     - (* AX done R *)
-      apply ax_done in H as (Hw & x & Heq & H).
-      intros.
-      specialize (Hk _ _ H); remember (k x) as K;
+      apply ax_done in H as (Hw & x & Heq & e & v & -> & HPost).
+      specialize (Hk _ _ _ HPost); remember (k x) as K;
         destruct Hk; try contradiction; subst.
       apply RStepA.
-      + rewrite Heq, bind_ret_l; try (exact (equ eq)).
-        apply H0.
+      + rewrite Heq, bind_ret_l; try (exact (equ eq)); auto.
       + split.
         * rewrite Heq, bind_ret_l.
-          now destruct H1.
+          now destruct H0.
         * intros t' w' TR.
-          apply (id_T (car_ (entailsF <( vis {φ} )>) (entailsF <( ⊥ )>))).          
-          cbn.
-          destruct H1.
-          apply H2.
+          apply (id_T (car_ (entailsF <( vis {φ} )>) (entailsF <( ⊥ )>))); cbn.
+          destruct H0.
+          apply H1.
           eapply ktrans_sbisim_ret with (t:=t0); auto.
     - (* vis φ *)
       destruct H0, H1; clear H0.
       destruct H1 as (t' & w' & TR).
-      apply RStepA.
-      + apply H. 
-      + split.
-        * apply can_step_bind_l with t' w'; auto.
-          destruct (H3 _ _ TR); try contradiction.
-          destruct H1.
-          inv H0; constructor.
-        * intros k_ w_ TRk.
-          apply ktrans_bind_inv in TRk as [(t0' & TR0 & Hd_ & Heq) | (x & w0 & TRt0 & Hd & TRk)].
-          -- (* [t0] steps and is not [Ret] *)
-            apply (fT_T (mequ_clos_car (KS:=KripkeSetoidEqu))).
-            cbn; eapply mequ_clos_ctor with (t1:=x <- t0';; k x) (w1:=w_); auto.
-            clear Heq k_.            
-            eapply (fTf_Tf (car_ <( |- vis φ )> <( |- ⊥ )>)).
-            apply in_bind_ctx1.
-            ++ rewrite unfold_entailsF.
-               now apply H2.
-            ++ intros.
-               apply (b_T (car_ <( |- vis φ )> <( |- ⊥ )>)).
-               cbn.
-               now apply Hk.
-          -- (* [t0] steps and is [Ret], contradiction *)
-            ddestruction Hd; subst;
-              specialize (H3 _ _ TRt0); ddestruction H3;
-              try contradiction;
-              destruct H1, H0;
-              rewrite can_step_bind in H1;
-              destruct H1 as [(? & ? & TRinv & ?) | (? & ? & TRinv & ?)];
-              now apply ktrans_stuck in TRinv.
+      apply RStepA; auto.
+      split.
+      + apply can_step_bind_l with t' w'; auto.
+        destruct (H3 _ _ TR); try contradiction.
+        destruct H1.
+        inv H0; constructor.
+      + intros k_ w_ TRk.
+        apply ktrans_bind_inv in TRk as
+            [(t0' & TR0 & Hd_ & Heq) | (x & w0 & TRt0 & Hd & TRk)].
+        * (* [t0] steps and is not [Ret] *)
+          apply (fT_T (mequ_clos_car (KS:=KripkeSetoidEqu))).
+          cbn; eapply mequ_clos_ctor with (t1:=x <- t0';; k x) (w1:=w_); auto.
+          clear Heq k_.            
+          eapply (fTf_Tf (car_ <( |- vis φ )> <( |- ⊥ )>)).
+          apply in_bind_ctx1.
+          -- rewrite unfold_entailsF; auto.             
+          -- intros.
+             apply (b_T (car_ <( |- vis φ )> <( |- ⊥ )>)); cbn; auto.
+        * (* [t0] steps and is [Ret], contradiction *)
+          ddestruction Hd; subst;
+            specialize (H3 _ _ TRt0); ddestruction H3;
+            try contradiction;
+            destruct H1, H0;
+            rewrite can_step_bind in H1;
+            destruct H1 as [(? & ? & TRinv & ?) | (? & ? & TRinv & ?)];
+            now apply ktrans_stuck in TRinv.
   Qed.
 
-  Lemma ag_iter{X I}: forall (k: I -> ctree E (I + X)) w (x: I) φ R,
+  (* [t] satisfies [φ] until it terminates with post-condition [R],
+     then forall x w, R x w -> k x, w satisfies [φ] forever. *)
+  Lemma ag_bind_vis{X Y}: forall (t: ctree E X)
+                          w (k: X -> ctree E Y) φ R,
+      <( t, w |= (vis φ) AU (AX finish R) )> ->
+      (forall (x: X) (e: E) (v: encode e), R e v x -> <( {k x}, {Obs e v} |= AG vis φ )>) ->
+      <( {x <- t ;; k x} , w |= AG vis φ )>.
+  Proof.
+    intros.
+    rewrite unfold_entailsF.
+    apply (ft_t (ag_bind_vis_ag φ R)).
+    cbn.
+    apply in_bind_ctx1; auto.
+  Qed.
+
+  Lemma ag_iter_vis{X I}: forall (k: I -> ctree E (I + X)) w (x: I) φ R,
       R x ->          (* Iterator invariant: [x] in [R] *)
       vis_with φ w -> (* Worlds invariant: [w = Obs e v /\ φ e v] *)
-      (forall (i: I) w,
+      (forall (i: I) (e: E) (v: encode e),
           R i ->
-          vis_with φ w ->
-          <( {k i}, w |= AX vis φ )> /\
-          <( {k i}, w |= vis φ AU AX done
-                      {fun (lr: I+X) (w: World E) =>
-                          exists i' : I, lr = inl i' /\ vis_with φ w /\ R i'})>) ->
+          φ e v ->
+          <( {k i}, {Obs e v} |= AX (vis φ AU AX finish
+                               {fun (e: E) (v: encode e) (lr: I+X) =>
+                                  exists i' : I, lr = inl i' /\ φ e v /\ R i'}))>) ->
       <( {iter k x}, w |= AG vis φ )>.
-  Proof.
+  Proof with auto with ctl.
     (* Coinduction steps *)
     intros.
     generalize dependent x.
     generalize dependent w.    
     coinduction RR CIH; intros.
-    apply RStepA; auto.
-    split.
+    apply RStepA...
+    split; inv H0.
     - (* can_step (iter k x) w *)
-      destruct (H1 _ _ H H0).
-      cdestruct H2.
+      specialize (H1 _ _ _ H H2) as HAX.
+      cdestruct HAX.
       destruct Hs as (k' & w' & TR).
-      destruct (H2 _ _ TR).
       rewrite sb_unfold_iter.
-      apply can_step_bind_l with k' (Obs e v); auto with ctl.
-    - intros t' w' TR.
+      specialize (HAX _ _ TR); cdestruct HAX.
+      + apply ax_done in H0 as (_ & ? & Heqt & e' & v' & -> & ? & -> & Hφ & HR).                
+        apply can_step_bind_l with t (Obs e' v')...
+      + destruct H3.
+        apply can_step_bind_l with t w...
+        inv H0...
+    - (* coinductive step *)
+      intros t' w' TR.
       rewrite unfold_iter in TR.
       apply ktrans_bind_inv in TR as [(t0' & TR0 & Hd_ & Heq) | (x' & w0 & TRt0 & Hd & TRk)].
       + (* [k x] steps *)
         rewrite Heq; clear Heq t'.
-        apply (ft_t (ag_bind_ag φ
-                       (fun (lr: I+X) (w: World E) =>
-                          exists i' : I, lr = inl i' /\ vis_with φ w /\ R i'))); cbn.
+        apply (ft_t (ag_bind_vis_ag φ
+                       (fun (e: E) (v: encode e) (lr: I+X) =>
+                          exists i' : I, lr = inl i' /\ φ e v /\ R i'))); cbn.
         apply in_bind_ctx1.
-        * destruct (H1 _ _ H H0).
-          rewrite ctl_au_ax in H3.
-          cdestruct H3.
-          -- apply ax_done in H3 as
-                 (? & lr & Heqk & ? & -> & _ & i).
-             rewrite Heqk in H2.
-             cdestruct H2.
-             destruct Hs as (Stuck & w_ & ?).
-             specialize (H2 _ _ H4); inv H2; inv H4.
-          -- cdestruct H3.
-             cdestruct H4.
-             specialize (H4 _ _ TR0).
-             apply H4.
-        * intros [l | r] wi (? & Hinv & ? & ?); inv Hinv.
+        * specialize (H1 _ _ _ H H2) as HAX.
+          cdestruct HAX...
+        * intros [l | r] e' v' (i & Hinv & Hφ & HR); inv Hinv.
           rewrite sb_guard.
-          apply CIH; auto.
-      + (* [k x] returns *)
-        destruct (H1 _ _ H H0).
-        cdestruct H2.
-        inv Hd; specialize (H2 _ _ TRt0); inv H2.
+          apply CIH...
+      + (* [k x] returns *)        
+        specialize (H1 _ _ _ H H2) as HAX.        
+        cdestruct HAX.
+        specialize (HAX _ _ TRt0).
+        apply au_stuck in HAX.
+        cdestruct HAX.
+        now apply can_step_stuck in Hs0.
+  Qed.
+  
+  Program Definition ag_bind_pure_clos{X Y} Post : mon (MP Y) :=
+    {| body R t w :=
+        bind_ctx1
+          (fun (t: ctree E X) => <( t, w |= pure AU AX done {fun x w => Post x /\ w = Pure })>)
+          (fun (k: X -> ctree E Y) => forall (x: X), Post x -> R (k x) Pure)
+          t
+    |}.
+  Next Obligation.
+    revert H0.
+    apply leq_bind_ctx1; intros.
+    apply in_bind_ctx1; eauto.
   Qed.
 
+  Lemma ag_bind_pure_ag{X Y} Post:
+      ag_bind_pure_clos (X:=X) (Y:=Y) Post <= cart <( |- pure )> <( |- ⊥ )>.
+  Proof.
+    apply Coinduction.
+    intros R t w; cbn.
+    apply (leq_bind_ctx1 _ _
+             (fun t => carF (entailsF <( pure )>) (entailsF <( ⊥ )>)
+                      (carT (entailsF <( pure )>) (entailsF <( ⊥ )>)
+                         (ag_bind_pure_clos Post) R) t w)). 
+    intros x Hx k Hk.
+    cinduction Hx.
+    - (* AX done R *)
+      apply ax_done in H as (Hw & x & Heq & HPost & ->). 
+      specialize (Hk _ HPost); remember (k x) as K;
+        destruct Hk; try contradiction; subst.
+      apply RStepA.
+      + rewrite Heq, bind_ret_l; try (exact (equ eq)); auto.
+      + split.
+        * rewrite Heq, bind_ret_l.
+          now destruct H0.
+        * intros t' w' TR.
+          apply (id_T (car_
+                         (entailsF <( now {fun w0 : World E => w0 = w} )>)
+                         (entailsF <( ⊥ )>))); cbn.
+          destruct H0.
+          apply H1.
+          eapply ktrans_sbisim_ret with (t:=t0); auto.
+    - (* pure *)
+      destruct H0, H1; clear H0.
+      destruct H1 as (t' & w' & TR).
+      apply RStepA; auto.
+      split.
+      + apply can_step_bind_l with t' w'; auto.
+        destruct (H3 _ _ TR); try contradiction.
+        destruct H1.
+        inv H0; constructor.
+      + intros k_ w_ TRk.
+        apply ktrans_bind_inv in TRk as
+            [(t0' & TR0 & Hd_ & Heq) | (x & w0 & TRt0 & Hd & TRk)].
+        * (* [t0] steps and is not [Ret] *)
+          apply (fT_T (mequ_clos_car (KS:=KripkeSetoidEqu))).
+          cbn; eapply mequ_clos_ctor with (t1:=x <- t0';; k x) (w1:=w_); auto.
+          clear Heq k_.            
+          eapply (fTf_Tf (car_ <( |- pure )> <( |- ⊥ )>)).
+          apply in_bind_ctx1.
+          -- rewrite unfold_entailsF; auto.             
+          -- intros.
+             apply (b_T (car_ <( |- pure )> <( |- ⊥ )>)); cbn; auto.
+        * (* [t0] steps and is [Ret], contradiction *)
+          ddestruction Hd; subst;
+            specialize (H3 _ _ TRt0); ddestruction H3;
+            try contradiction;
+            destruct H1, H0;
+            rewrite can_step_bind in H1;
+            destruct H1 as [(? & ? & TRinv & ?) | (? & ? & TRinv & ?)];
+            now apply ktrans_stuck in TRinv.
+  Qed.
+
+  (* [t] satisfies [φ] until it terminates with post-condition [R],
+     then forall x w, R x w -> k x, w satisfies [φ] forever. *)
+  Lemma ag_bind_pure{X Y}: forall (t: ctree E X)
+                          w (k: X -> ctree E Y) R,
+      <( t, w |= pure AU AX done {fun x w => R x /\ w = Pure })> ->
+      (forall (x: X), R x -> <( {k x}, {Pure} |= AG pure )>) ->
+      <( {x <- t ;; k x} , w |= AG pure )>.
+  Proof.
+    intros.
+    rewrite unfold_entailsF.
+    apply (ft_t (ag_bind_pure_ag R)).
+    cbn.
+    apply in_bind_ctx1; auto.
+  Qed.
+  
+  Lemma ag_iter_pure{X I}: forall (k: I -> ctree E (I + X)) (x: I) (R: I -> Prop),
+      R x ->          (* Iterator invariant: [x] in [R] *)
+      (forall (i: I),
+          R i ->
+          <( {k i}, Pure |= AX (pure AU AX done
+                               {fun (lr: I+X) (w: World E) =>
+                                  exists i' : I, lr = inl i' /\ R i' /\ w = Pure}))>) ->
+      <( {iter k x}, Pure |= AG pure )>.
+  Proof with auto with ctl.
+    (* Coinduction steps *)
+    intros * HR H.
+    generalize dependent x.
+    coinduction RR CIH; intros.
+    apply RStepA...
+    split.
+    - (* can_step (iter k x) w *)
+      specialize (H _ HR) as HAX.
+      cdestruct HAX.
+      destruct Hs as (k' & w' & TR).
+      rewrite sb_unfold_iter.
+      specialize (HAX _ _ TR); cdestruct HAX.
+      + apply ax_done in H0 as (_ & ? & Heqt & i & -> & HR' & ->). 
+        apply can_step_bind_l with t Pure...
+      + destruct H1.
+        inv H0.
+        apply can_step_bind_l with t Pure...
+    - (* coinductive step *)
+      intros t' w' TR.
+      rewrite unfold_iter in TR.
+      apply ktrans_bind_inv in TR as [(t0' & TR0 & Hd_ & Heq) | (x' & w0 & TRt0 & Hd & TRk)].
+      + (* [k x] steps *)
+        rewrite Heq; clear Heq t'.
+        apply (ft_t (ag_bind_pure_ag
+                       (fun (lr: I+X) => exists i' : I, lr = inl i' /\ R i'))); cbn.
+        apply in_bind_ctx1.
+        * specialize (H _ HR) as HAX.
+          cdestruct HAX.
+          specialize (HAX _ _ TR0).
+          assert(Hdeq:
+                  equiv_ctl (X:= I+X)
+                  <(done {fun (x0 : I + X) (w : World E) =>
+                            (exists i' : I, x0 = inl i' /\ R i') /\ w = Pure})>
+                  <(done {fun (x0 : I + X) (w : World E) =>
+                            exists i' : I, x0 = inl i' /\ R i' /\ w = Pure})>);
+            [|rewrite Hdeq]...
+          split; intros H'; inv H'; destruct H0 as [? Hb].
+          -- destruct H0 as (i & -> & ?); constructor; eauto.
+          -- inv Hb.
+          -- destruct Hb as (-> & ? & ?); constructor; eauto.
+          -- destruct Hb as (-> & ? & Hinv); inv Hinv.
+        * intros ? (i & -> & HR').
+          rewrite sb_guard.
+          apply CIH...
+      + (* [k x] returns *)        
+        specialize (H _ HR) as HAX.        
+        cdestruct HAX.
+        specialize (HAX _ _ TRt0).
+        apply au_stuck in HAX.
+        cdestruct HAX.
+        now apply can_step_stuck in Hs0.
+  Qed.
 End BindLemmas.
+
+(*| Combinators for [interp_state] |*)
+Section CtlAgState.
+  Context {E F S: Type} {HE: Encode E} {HF: Encode F}
+    (h: E ~> stateT S (ctree F)).
+
+  Theorem ag_bind_state_l{X Y}: forall s w (t: ctree E Y) (k: Y -> ctree E X) φ,
+      <( {interp_state h t s}, w |= AG now φ )> ->
+      <( {interp_state h (x <- t ;; k x) s}, w |= AG now φ )>.
+  Proof.
+    intros.
+    rewrite interp_state_bind.
+    now apply ag_bind_l.
+  Qed.
+
+  Theorem ag_bind_state_vis{X Y}: forall s (t: ctree E Y) (k: Y -> ctree E X) w φ R,
+      <( {interp_state h t s}, w |= (vis φ) AU (AX finish R) )> ->
+      (forall (e: F) (v: encode e) (y: Y) (s: S),
+          R e v (y, s) ->
+          <( {interp_state h (k y) s}, {Obs e v} |= AG vis φ )>) ->
+      <( {interp_state h (x <- t ;; k x) s} , w |= AG vis φ )>.
+  Proof.
+    intros.
+    rewrite interp_state_bind.
+    apply ag_bind_vis with (R:=R); auto.
+    intros [y s'] w' Hr; auto.
+  Qed.
+
+  Theorem ag_bind_state_pure{X Y}: forall s (t: ctree E Y) w (k: Y -> ctree E X) R,
+      <( {interp_state h t s}, w |= pure AU (AX done {fun x w => R x /\ w = Pure}) )> ->
+      (forall (y: Y) (s: S), R (y, s) -> <( {interp_state h (k y) s}, Pure |= AG pure )>) ->
+      <( {interp_state h (x <- t ;; k x) s}, w |= AG pure )>.
+  Proof.
+    intros.
+    rewrite interp_state_bind.
+    apply ag_bind_pure with (R:=R); auto.
+    intros [y s'] Hr; auto.
+  Qed.
+  
+  Theorem ag_iter_state_vis{X I}: forall s (k: I -> ctree E (I + X)) w (x: I) φ R,
+      R (x, s) ->     (* Iterator invariant: [x] in [R] *)
+      vis_with φ w -> (* Worlds invariant: [w = Obs e v /\ φ e v] *)
+      (forall (x: I) (s: S) (e: F) (v: encode e),
+          R (x, s) ->
+          φ e v ->
+          <( {interp_state h (k x) s}, {Obs e v} |= AX (vis φ AU AX finish
+             {fun (e: F) (v: encode e) (lr: (I+X) * S) =>
+                exists (i' : I) (s': S), lr = (inl i', s') /\ φ e v /\ R (i', s')}))>) ->
+      <( {interp_state h (iter k x) s}, w |= AG vis φ )>.
+  Proof with auto with ctl.
+    intros.
+    rewrite interp_state_unfold_iter.
+    inv H0.
+    generalize dependent x.
+    generalize dependent e.
+    generalize dependent s.
+    coinduction RR CIH; intros.
+    apply RStepA; [apply ctl_vis; now constructor|].
+    split.
+    - specialize (H1 _ _ _ _ H H2).
+      cdestruct H1.
+      destruct Hs as (t' & w' & TR).
+      specialize (H1 _ _ TR).
+      apply can_step_bind_l with t' w'; auto.
+      cdestruct H1.
+      + now apply ax_done in H0 as (? & ?).
+      + inv H0; constructor.
+    - intros t' w' TR.
+      apply ktrans_bind_inv in TR as [(t0' & TR0 & Hd_ & Heq) | (x' & w0 & TRt0 & Hd & TRk)].
+      + (* [k x] steps *)
+        rewrite Heq; clear Heq t'.
+        apply (ft_t (ag_bind_vis_ag φ
+                       (fun (e: F) (v: encode e) (lr: (I+X) * S) =>
+                          exists (i': I) (s': S), lr = (inl i', s') /\ φ e v /\ R (i', s')))); cbn.
+        apply in_bind_ctx1.
+        * specialize (H1 _ _ _ _ H H2) as HAX.
+          cdestruct HAX.
+          specialize (HAX _ _ TR0).
+          apply HAX.
+        * intros (lr' & s_) e' v' (i & s' & Hinv & Hφ & HR'); inv Hinv.
+          rewrite sb_guard.
+          setoid_rewrite interp_state_unfold_iter.
+          apply CIH...
+      + (* [k x] returns *)        
+        specialize (H1 _ _ _ _ H H2) as HAX.        
+        cdestruct HAX.
+        specialize (HAX _ _ TRt0).
+        apply au_stuck in HAX.
+        cdestruct HAX.
+        now apply can_step_stuck in Hs0.
+  Qed.        
+    
+End CtlAgState.
